Modules.thy
@@ -26,9 +26,9 @@ lemma Rep_type_Type: "Rep_type (Type (T::'a::prog_type itself)) =
   unfolding Type_def by (subst Abs_type_inverse, auto)
 
 
-record procedure_type =
+(* record procedure_type =
   pt_argtype :: "type"
-  pt_returntype :: "type"
+  pt_returntype :: "type" *)
 
 datatype 'a procedure =
   Proc 'a
@@ -49,29 +49,29 @@ datatype lambda =
   p_return :: 'c *)
 
 
-datatype procedure_type_open = 
-   ProcTSimple procedure_type
- | ProcTFun procedure_type_open procedure_type_open
- | ProcTPair procedure_type_open procedure_type_open
+datatype 'program_type procedure_type_open = 
+   ProcTSimple 'program_type
+ | ProcTFun "'program_type procedure_type_open" "'program_type procedure_type_open"
+ | ProcTPair "'program_type procedure_type_open" "'program_type procedure_type_open"
  | ProcTUnit
 
 locale modules =
-  (* 'program = type of programs *)
-  fixes well_typed_program :: "(procedure_type_open list \<Rightarrow> 'program procedure \<Rightarrow> procedure_type_open \<Rightarrow> bool)
-                             \<Rightarrow> procedure_type_open list \<Rightarrow> 'program \<Rightarrow> procedure_type \<Rightarrow> bool"
-    and proc_list :: "'program \<Rightarrow> 'program procedure list"
+  (* 'program = type of programs, 'program_type = type of programs *)
+  fixes proc_list :: "'program \<Rightarrow> 'program procedure list"
     and proc_size :: "'program procedure \<Rightarrow> nat"
     and proc_update' :: "'program \<Rightarrow> 'program procedure list \<Rightarrow> 'program"
+    and well_typed_program :: "('program_type procedure_type_open list \<Rightarrow> 'program procedure \<Rightarrow> 'program_type procedure_type_open \<Rightarrow> bool)
+                             \<Rightarrow> 'program_type procedure_type_open list \<Rightarrow> 'program \<Rightarrow> 'program_type \<Rightarrow> bool"
   assumes proc_size_Proc: "y \<in> set (proc_list x) \<Longrightarrow> proc_size y < proc_size (Proc x)" 
       and proc_size_ProcAppl[simp]: "proc_size (ProcAppl s t) = proc_size s + proc_size t + 1"
       and proc_size_ProcPair[simp]: "proc_size (ProcPair s t) = proc_size s + proc_size t + 1"
       and proc_size_ProcUnpair[simp]: "proc_size (ProcUnpair b s) = proc_size s + 1"
       and proc_size_ProcAbs[simp]: "proc_size (ProcAbs s) = proc_size s + 1"
       and well_typed_program_mono[mono]: "wt \<le> wt' \<Longrightarrow> well_typed_program wt E p T \<longrightarrow> well_typed_program wt' E p T"
-      and well_typed_program_simple: "well_typed_program wt E p T \<Longrightarrow> \<forall>pc\<in>set(proc_list pc). \<exists>T'. wt E pc (ProcTSimple T')"
+      and well_typed_program_simple: "well_typed_program wt E p T \<Longrightarrow> \<forall>pc\<in>set(proc_list p). \<exists>T'. wt E pc (ProcTSimple T')"
       and proc_update'_list: "length l = length (proc_list proc) \<Longrightarrow> proc_list (proc_update' proc l) = l"
       and proc_update'_self[simp]: "proc_update' proc (proc_list proc) = proc"
-      and proc_update'_twice[simp]: "proc_update' (proc_update' proc l) l' = proc_update' proc l'"
+      and proc_update'_twice: "length l = length (proc_list proc) \<Longrightarrow> length l' = length (proc_list proc) \<Longrightarrow> proc_update' (proc_update' proc l) l' = proc_update' proc l'"
 begin
 
 
@@ -112,8 +112,8 @@ proof -
   have len: "length (proc_list a) = length (proc_list c)" 
     using assms unfolding same_shape_def by auto
   moreover have "a = proc_update' c (proc_list a)" 
-    apply (subst a, subst b) 
-    by simp
+    apply (subst a, subst b)
+    using assms(2) len proc_update'_twice same_shape_def by blast
   ultimately show ?thesis
     unfolding same_shape_def
     by simp
@@ -124,7 +124,8 @@ proof -
   have a: "a = proc_update' b (proc_list a)"
     using assms unfolding same_shape_def by auto
   have "b = proc_update' a (proc_list b)"
-    apply (subst a) by simp
+    apply (subst a)
+    using assms modules.proc_update'_twice modules_axioms same_shape_def by fastforce
   then show ?thesis
     using assms
     unfolding same_shape_def
@@ -137,7 +138,7 @@ lemma same_shape_update'L[simp]: "length (proc_list p) = length l \<Longrightarr
 
 lemma same_shape_update'R[simp]: "length (proc_list p) = length l \<Longrightarrow> same_shape p (proc_update' p l)"
   unfolding same_shape_def
-  by (simp add: proc_update'_list)
+  by (simp add: proc_update'_list proc_update'_twice)
 
 lemma same_shape_mapL[simp]: "same_shape (proc_map f p) p"
   unfolding proc_map_def by simp
@@ -198,7 +199,7 @@ lemma proc_relation_nth_mono[mono]:
 (* lemma wf_subterm_relation[simp]: "wf subterm_relation" using proc_set_wellfounded unfolding subterm_relation_def . *)
 
 
-inductive well_typed :: "procedure_type_open list \<Rightarrow> 'program procedure \<Rightarrow> procedure_type_open \<Rightarrow> bool"
+inductive well_typed :: "'program_type procedure_type_open list \<Rightarrow> 'program procedure \<Rightarrow> 'program_type procedure_type_open \<Rightarrow> bool"
   where wt_ProcRef: "i<length E \<Longrightarrow> E!i = T \<Longrightarrow> well_typed E (ProcRef i) T"
 | wt_ProcAppl: "well_typed E p (ProcTFun T U) \<Longrightarrow>
   well_typed E q T \<Longrightarrow>
@@ -421,7 +422,7 @@ qed auto
 
 abbreviation "ProcT == Fun (Atom 0) (Atom 0)"
 
-fun typ_conv :: "procedure_type_open \<Rightarrow> lambda_type" where
+fun typ_conv :: "'b procedure_type_open \<Rightarrow> lambda_type" where
   "typ_conv (ProcTSimple _) = ProcT"
 | "typ_conv ProcTUnit = ProcT"
 | "typ_conv (ProcTFun T U) = Fun (typ_conv T) (typ_conv U)"
@@ -842,7 +843,7 @@ proof -
   proof -
     have hybi: "hyb i = proc_update' s (proc_list (hyb i))" 
       unfolding hyb_def
-      by (metis proc_update'_self proc_update'_twice)
+      using assms proc_relation_def same_shape_def same_shape_update'L by auto
     have len': "length (take i (proc_list s') @ drop i (proc_list s)) = proc_length s"
       using assms list_all2_lengthD proc_relation_def by fastforce
     have len: "proc_length (hyb i) = proc_length s"
@@ -1292,7 +1293,7 @@ proof -
     qed}
   thus "diamond par_beta"
     unfolding diamond_def commute_def square_def by auto
-qed
+qed                                                                                                                    
 
 
 theorem beta_confluent: "confluent beta_reduce_proc"
